# Quardic Equation

> here is an example of using the quadratic formula12. Suppose you want to solve this equation: 5x²+6x+1=0. First, you identify the values of a, b, and c. In this case, a=5, b=6, and c=1. Then, you plug these values into the formula:

> (-b±√(b²-4ac))/(2a)

> and simplify:

* `(-6±√(6²-4*5*1))/(2*5)`

* `(-6±√(36-20))/10`

* `(-6±√16)/10`

* `(-6±4)/10`

> Now you have two possible solutions:

> x=(-6+4)/10=-0.2

or

* `x=(-6-4)/10=-1.`

> You can check your answers by plugging them back into the original equation. Do you have any questions?
